\chapter{Propositional Logic}
\section{The Language of Propositional Logic}
\begin{definition}
  Let $V$ be a countably infinite set, whose elements are called
  \emph{propositional variables}.
  We define the set of \emph{formulas} as the minimal set of strings on
  the alphabet $V \cup \{\neg, \to, (, )\}$ satisfying the following
  properties.
  \begin{enumerate}
    \item Each propositional variable in $V$ is a formula on $V$.
    \item If $\alpha$ is a formula, then so is $\neg\alpha$.
    \item If $\alpha$ and $\beta$ are formulas, then so is
    $(\alpha \to \beta)$.
  \end{enumerate}
\end{definition}

\section{Truth Assignment}
\begin{definition}
  A \emph{truth assignment} is a function $\tau: V \to \{0, 1\}$, and it can be
  extended to have its domain the set of formulas as follows.
  \begin{enumerate}
    \item $\tau(\neg\alpha) = 1 - \tau(\alpha)$ for any formula $\alpha$.
    \item $\tau((\alpha \to \beta)) = 1 - \tau(\alpha)
    (1 - \tau(\beta))$ for any formulas $\alpha$ and $\beta$.
  \end{enumerate}
\end{definition}

\begin{definition}
  We say that a truth assignment $\tau$ \emph{satisfies} a formula $\alpha$
  if $\tau(\alpha) = 1$.
  Also, we say that $\tau$ \emph{satisfies} a set $\Sigma$ of formulas if it
  satisfies each formula in $\Sigma$.
\end{definition}

\begin{definition}
  Let $\Gamma$ be a set of formulas and let $\alpha$ be a formula.
  We say that $\Gamma$ \emph{tautologically implies} $\alpha$, denoted by
  $\Gamma \vDash \alpha$, if every truth assignment satisfying $\Gamma$
  also satisfies $\alpha$.
\end{definition}

\section{Proof System}
\begin{definition}
  The collection $\Lambda$ of \emph{axioms} consists of the formulas listed
  below, where $\alpha, \beta, \gamma$ are formulas.
  \begin{enumerate}[leftmargin=3.5em]
    \item[(A1)] $\alpha \to (\beta \to \alpha)$.
    \item[(A2)] $(\alpha \to (\beta \to \gamma)) \to
    ((\alpha \to \beta) \to (\alpha \to \gamma))$.
    \item[(A3)] $(\neg \beta \to \neg \alpha) \to (\alpha \to \beta)$.
  \end{enumerate}
\end{definition}

\begin{definition}
  A \emph{proof} of a formula $\alpha$ from a collection $\Gamma$ of formulas
  is a sequence of formulas
  \begin{equation*}
    (\alpha_1, \alpha_2, \dots, \alpha_n)
  \end{equation*}
  satisfying the following properties.
  \begin{enumerate}
    \item $\alpha_n = \alpha$.
    \item For $k \in \{1, 2, \dots, n\}$, either
    $\alpha_k \in \Lambda \cup \Gamma$ or there exist
    $i, j \in \{1, 2, \dots, k-1\}$ with $\alpha_j = \alpha_i \to \alpha_k$.
  \end{enumerate}
  If there exists a proof of $\varphi$ from $\Gamma$, we write
  $\Gamma \vdash \varphi$.
  If $\varnothing \vdash \varphi$, we write $\vdash \varphi$ for short.
\end{definition}

\begin{theorem}[Law of Identity]
  \label{thm:identity}
  For any formula $\alpha$, we have $\vdash \alpha \to \alpha$.
\end{theorem}
\begin{proof}
  We have a proof of $\alpha \to \alpha$ as follows.
  \begin{enumerate}[(1)]
    \item $(\alpha \to ((\alpha \to \alpha) \to \alpha)) \to
    ((\alpha \to (\alpha \to \alpha)) \to (\alpha \to \alpha))$.
    \hfill (A2)
    \item $\alpha \to ((\alpha \to \alpha) \to \alpha)$. \hfill (A1)
    \item $(\alpha \to (\alpha \to \alpha)) \to (\alpha \to \alpha)$.
    \hfill (1, 2)
    \item $\alpha \to (\alpha \to \alpha)$. \hfill (A1)
    \item $\alpha \to \alpha$. \hfill (3, 4)
  \end{enumerate}
  Thus, we can conclude that $\vdash \alpha \to \alpha$.
\end{proof}

\begin{theorem}[Duns Scotus Law]
  \label{thm:contradiction}
  For any formula $\alpha$ and $\beta$, we have
  $\vdash \neg\alpha \to (\alpha \to \beta)$.
\end{theorem}
\begin{proof}
  We have a proof of $\neg\alpha \to (\alpha \to \beta)$ as follows.
  \begin{enumerate}[(1)]
    \item $((\neg\beta \to \neg\alpha) \to (\alpha \to \beta))
    \to (\neg\alpha \to ((\neg\beta \to \neg\alpha) \to (\alpha \to \beta)))$.
    \hfill (A1)
    \item $(\neg\beta \to \neg\alpha) \to (\alpha \to \beta)$. \hfill (A3)
    \item $\neg\alpha \to ((\neg\beta \to \neg\alpha) \to (\alpha \to \beta))$.
    \hfill (1, 2)
    \item $(\neg\alpha \to ((\neg\beta \to \neg\alpha) \to (\alpha \to \beta)))
    \to ((\neg\alpha \to (\neg\beta \to \neg\alpha))
    \to (\neg\alpha \to (\alpha \to \beta)))$. \\ \hbox{} \hfill (A2)
    \item $(\neg\alpha \to (\neg\beta \to \neg\alpha))
    \to (\neg\alpha \to (\alpha \to \beta))$. \hfill (3, 4)
    \item $\neg\alpha \to (\neg\beta \to \neg\alpha)$. \hfill (A1)
    \item $\neg\alpha \to (\alpha \to \beta)$. \hfill (5, 6)
  \end{enumerate}
  Thus, we can conclude that $\vdash \neg\alpha \to (\alpha \to \beta)$.
\end{proof}

\begin{theorem}[Modus Ponens]
  \label{thm:modus-ponens}
  For any formula $\alpha$ and $\beta$, we have
  $\vdash \alpha \to ((\alpha \to \beta) \to \beta)$.
\end{theorem}
\begin{proof}
  We have a proof of $\alpha \to ((\alpha \to \beta) \to \beta)$ as follows.
  \begin{enumerate}[(1)]
    \item $(\alpha \to \beta) \to (\alpha \to \beta)$.
    \hfill (\Cref{thm:identity})
    \item $((\alpha \to \beta) \to (\alpha \to \beta)) \to
    (((\alpha \to \beta) \to \alpha) \to ((\alpha \to \beta) \to \beta))$.
    \hfill (A2)
    \item $((\alpha \to \beta) \to \alpha) \to ((\alpha \to \beta) \to \beta)$.
    \hfill (1, 2)
    \item $(((\alpha \to \beta) \to \alpha) \to ((\alpha \to \beta) \to \beta))
    \to (\alpha \to (((\alpha \to \beta) \to \alpha) \to ((\alpha \to \beta)
    \to \beta)))$. \hfill (A1)
    \item $\alpha \to (((\alpha \to \beta) \to \alpha) \to ((\alpha \to \beta)
    \to \beta))$. \hfill (3, 4)
    \item $(\alpha \to (((\alpha \to \beta) \to \alpha) \to ((\alpha \to \beta)
    \to \beta))) \to ((\alpha \to ((\alpha \to \beta) \to \alpha)) \to (\alpha
    \to ((\alpha \to \beta) \to \beta)))$. \hfill (A2)
    \item $(\alpha \to ((\alpha \to \beta) \to \alpha)) \to (\alpha \to
    ((\alpha \to \beta) \to \beta))$. \hfill (5, 6)
    \item $\alpha \to ((\alpha \to \beta) \to \alpha)$. \hfill (A1)
    \item $\alpha \to ((\alpha \to \beta) \to \beta)$. \hfill (7, 8)
  \end{enumerate}
  Thus, we can conclude that
  $\vdash \alpha \to ((\alpha \to \beta) \to \beta)$.
\end{proof}

\begin{theorem}[Hypothetical Syllogism]
  \label{thm:syl}
  For any formulas $\alpha$, $\beta$ and $\gamma$, we have
  $\vdash (\beta \to \gamma) \to ((\alpha \to \beta) \to (\alpha \to \gamma))$.
\end{theorem}
\begin{proof}
  We have a proof of $(\beta \to \gamma) \to ((\alpha \to \beta) \to (\alpha
  \to \gamma))$ as follows.
  \begin{enumerate}[(1)]
    \item $(\alpha \to (\beta \to \gamma)) \to ((\alpha \to \beta) \to
    (\alpha \to \gamma))$. \hfill (A2)
    \item $((\alpha \to (\beta \to \gamma)) \to ((\alpha \to \beta) \to
    (\alpha \to \gamma))) \to ((\beta \to \gamma) \to ((\alpha \to (\beta \to
    \gamma)) \to ((\alpha \to \beta) \to (\alpha \to \gamma))))$. \hfill (A1)
    \item $(\beta \to \gamma) \to ((\alpha \to (\beta \to \gamma)) \to
    ((\alpha \to \beta) \to (\alpha \to \gamma)))$. \hfill (1, 2)
    \item $((\beta \to \gamma) \to ((\alpha \to (\beta \to \gamma)) \to
    ((\alpha \to \beta) \to (\alpha \to \gamma)))) \to (((\beta \to \gamma) \to
    (\alpha \to (\beta \to \gamma))) \to ((\beta \to \gamma) \to
    ((\alpha \to \beta) \to (\alpha \to \gamma))))$. \hfill (A2)
    \item $((\beta \to \gamma) \to (\alpha \to (\beta \to \gamma))) \to ((\beta
    \to \gamma) \to ((\alpha \to \beta) \to (\alpha \to \gamma)))$.
    \hfill (3, 4)
    \item $(\beta \to \gamma) \to (\alpha \to (\beta \to \gamma))$. \hfill (A1)
    \item $(\beta \to \gamma) \to ((\alpha \to \beta) \to
    (\alpha \to \gamma))$. \hfill (5, 6)
  \end{enumerate}
  Thus, we can conclude that
  $\vdash (\beta \to \gamma) \to ((\alpha \to \beta) \to (\alpha \to \gamma))$.
\end{proof}

\begin{theorem}[Clavius's Law]
  \label{thm:clavius}
  For any formula $\alpha$, we have $\vdash (\neg\alpha \to \alpha) \to
  \alpha$.
\end{theorem}
\begin{proof}
  We have a proof of $(\neg\alpha \to \alpha) \to \alpha$ as follows.
  \begin{enumerate}[(1)]
    \item $(\neg\alpha \to (\alpha \to \neg(\neg\alpha \to \alpha))) \to
    ((\neg\alpha \to \alpha) \to (\neg\alpha \to \neg(\neg\alpha \to
    \alpha)))$. \hfill (A2)
    \item $\neg\alpha \to (\alpha \to \neg(\neg\alpha \to \alpha))$.
    \hfill (\Cref{thm:contradiction})
    \item $(\neg\alpha \to \alpha) \to (\neg\alpha \to \neg(\neg\alpha \to
    \alpha))$. \hfill (1, 2)
    \item $(\neg\alpha \to \neg(\neg\alpha \to \alpha)) \to ((\neg\alpha \to
    \alpha) \to \alpha)$. \hfill (A3)
    \item $((\neg\alpha \to \neg(\neg\alpha \to \alpha)) \to ((\neg\alpha \to
    \alpha) \to \alpha)) \to (((\neg\alpha \to \alpha) \to (\neg\alpha \to
    \neg(\neg\alpha \to \alpha))) \to ((\neg\alpha \to \alpha) \to ((\neg\alpha
    \to \alpha) \to \alpha)))$. \hfill (\Cref{thm:syl})
    \item $((\neg\alpha \to \alpha) \to (\neg\alpha \to \neg(\neg\alpha \to
    \alpha))) \to ((\neg\alpha \to \alpha) \to ((\neg\alpha \to \alpha) \to
    \alpha))$. \hfill (4, 5)
    \item $(\neg\alpha \to \alpha) \to ((\neg\alpha \to \alpha) \to \alpha)$.
    \hfill (3, 6)
    \item $((\neg\alpha \to \alpha) \to ((\neg\alpha \to \alpha) \to \alpha))
    \to (((\neg\alpha \to \alpha) \to (\neg\alpha \to \alpha)) \to
    ((\neg\alpha \to \alpha) \to \alpha))$. \hfill (A2)
    \item $((\neg\alpha \to \alpha) \to (\neg\alpha \to \alpha)) \to
    ((\neg\alpha \to \alpha) \to \alpha)$ \hfill (7, 8)
    \item $(\neg\alpha \to \alpha) \to (\neg\alpha \to \alpha)$.
    \hfill (\Cref{thm:identity})
    \item $(\neg\alpha \to \alpha) \to \alpha$. \hfill (9, 10)
  \end{enumerate}
  Thus, we can conclude that $\vdash (\neg\alpha \to \alpha) \to \alpha$.
\end{proof}

\begin{theorem}[Elimination of Double Negation]
  \label{thm:dn-elim}
  For any formula $\alpha$, we have $\vdash \neg\neg\alpha \to \alpha$.
\end{theorem}
\begin{proof}
  We have a proof of $\neg\neg\alpha \to \alpha$ as follows.
  \begin{enumerate}[(1)]
    \item $((\neg\alpha \to \alpha) \to \alpha) \to ((\neg\neg\alpha \to
    (\neg\alpha \to \alpha)) \to (\neg\neg\alpha \to \alpha))$.
    \hfill (\Cref{thm:syl})
    \item $(\neg\alpha \to \alpha) \to \alpha$. \hfill (\Cref{thm:clavius})
    \item $(\neg\neg\alpha \to (\neg\alpha \to \alpha)) \to (\neg\neg\alpha \to
    \alpha)$. \hfill (1, 2)
    \item $\neg\neg\alpha \to (\neg\alpha \to \alpha)$.
    \hfill (\Cref{thm:contradiction})
    \item $\neg\neg\alpha \to \alpha$. \hfill (3, 4)
  \end{enumerate}
  Thus, we can conclude that $\vdash \neg\neg\alpha \to \alpha$.
\end{proof}

\begin{theorem}[Introduction of Double Negation]
  \label{thm:dn-intro}
  For any formula $\alpha$, we have $\vdash \alpha \to \neg\neg\alpha$.
\end{theorem}
\begin{proof}
  We have a proof of $\alpha \to \neg\neg\alpha$ as follows.
  \begin{enumerate}[(1)]
    \item $(\neg\neg\neg\alpha \to \neg\alpha) \to (\alpha \to
    \neg\neg\alpha)$. \hfill (A3)
    \item $\neg\neg\neg\alpha \to \neg\alpha$. \hfill (\Cref{thm:dn-elim})
    \item $\alpha \to \neg\neg\alpha$. \hfill (1, 2)
  \end{enumerate}
  Thus, we can conclude that $\vdash \alpha \to \neg\neg\alpha$.
\end{proof}

\begin{theorem}[Law of Contraposition]
  \label{thm:contraposition}
  For any formulas $\alpha$ and $\beta$, we have $\vdash (\alpha \to \beta) \to
  (\neg\beta \to \neg\alpha)$.
\end{theorem}
\begin{proof}
  We have a proof of $(\alpha \to \beta) \to (\neg\beta \to \neg\alpha)$
  as follows.
  \begin{enumerate}[(1)]
    \item $(\beta \to \neg\neg\beta) \to ((\neg\neg\alpha \to \beta) \to
    (\neg\neg\alpha \to \neg\neg\beta))$. \hfill (\Cref{thm:syl})
    \item $\beta \to \neg\neg\beta$. \hfill (\Cref{thm:dn-intro})
    \item $(\neg\neg\alpha \to \beta) \to (\neg\neg\alpha \to \neg\neg\beta)$.
    \hfill (1, 2)
    \item $((\neg\neg\alpha \to \beta) \to (\neg\neg\alpha \to \neg\neg\beta))
    \to ((\alpha \to \beta) \to ((\neg\neg\alpha \to \beta) \to (\neg\neg\alpha
    \to \neg\neg\beta)))$. \hfill (A1)
    \item $(\alpha \to \beta) \to ((\neg\neg\alpha \to \beta) \to
    (\neg\neg\alpha \to \neg\neg\beta))$. \hfill (3, 4)
    \item $(\alpha \to \beta) \to ((\neg\neg\alpha \to \alpha) \to
    (\neg\neg\alpha \to \beta))$. \hfill (\Cref{thm:syl})
    \item $((\alpha \to \beta) \to ((\neg\neg\alpha \to \alpha) \to
    (\neg\neg\alpha \to \beta))) \to (((\alpha \to \beta) \to (\neg\neg\alpha
    \to \alpha)) \to ((\alpha \to \beta) \to (\neg\neg\alpha \to \beta)))$.
    \hfill (A2)
    \item $((\alpha \to \beta) \to (\neg\neg\alpha \to \alpha)) \to ((\alpha
    \to \beta) \to (\neg\neg\alpha \to \beta))$. \hfill (6, 7)
    \item $(\neg\neg\alpha \to \alpha) \to ((\alpha \to \beta) \to
    (\neg\neg\alpha \to \alpha))$. \hfill (A1)
    \item $\neg\neg\alpha \to \alpha$. \hfill (\Cref{thm:dn-elim})
    \item $(\alpha \to \beta) \to (\neg\neg\alpha \to \alpha)$. \hfill (9, 10)
    \item $(\alpha \to \beta) \to (\neg\neg\alpha \to \beta)$. \hfill (8, 11)
    \item $((\alpha \to \beta) \to ((\neg\neg\alpha \to \beta) \to
    (\neg\neg\alpha \to \neg\neg\beta))) \to (((\alpha \to \beta) \to
    (\neg\neg\alpha \to \beta)) \to ((\alpha \to \beta) \to (\neg\neg\alpha \to
    \neg\neg\beta)))$. \hfill (A2)
    \item $((\alpha \to \beta) \to (\neg\neg\alpha \to \beta)) \to ((\alpha \to
    \beta) \to (\neg\neg\alpha \to \neg\neg\beta))$. \hfill (5, 13)
    \item $(\alpha \to \beta) \to (\neg\neg\alpha \to \neg\neg\beta)$.
    \hfill (12, 14)
    \item $((\neg\neg\alpha \to \neg\neg\beta) \to (\neg\beta \to \neg\alpha))
    \to (((\alpha \to \beta) \to (\neg\neg\alpha \to \neg\neg\beta)) \to
    ((\alpha \to \beta) \to (\neg\beta \to \neg\alpha)))$.
    \hfill (\Cref{thm:syl})
    \item $(\neg\neg\alpha \to \neg\neg\beta) \to (\neg\beta \to \neg\alpha)$.
    \hfill (A3)
    \item $((\alpha \to \beta) \to (\neg\neg\alpha \to \neg\neg\beta)) \to
    ((\alpha \to \beta) \to (\neg\beta \to \neg\alpha))$. \hfill (16, 17)
    \item $(\alpha \to \beta) \to (\neg\beta \to \neg\alpha)$. \hfill (15, 18)
  \end{enumerate}
  Thus, we can conclude that
  $\vdash (\alpha \to \beta) \to (\neg\beta \to \neg\alpha)$.
\end{proof}

\begin{theorem}
  For any formulas $\alpha$ and $\beta$, we have $\vdash \alpha \to (\neg\beta
  \to \neg(\alpha \to \beta))$.
\end{theorem}
\begin{proof}
  We have a proof of $\alpha \to (\neg\beta \to \neg(\alpha \to \beta))$
  as follows.
  \begin{enumerate}[(1)]
    \item $((\alpha \to \beta) \to \beta) \to (\neg\beta \to \neg(\alpha \to
    \beta))$. \hfill (\Cref{thm:contraposition})
    \item $(((\alpha \to \beta) \to \beta) \to (\neg\beta \to \neg(\alpha \to
    \beta))) \to (\alpha \to (((\alpha \to \beta) \to \beta) \to (\neg\beta \to
    \neg(\alpha \to \beta))))$. \hfill (A1)
    \item $\alpha \to (((\alpha \to \beta) \to \beta) \to (\neg\beta \to
    \neg(\alpha \to \beta)))$. \hfill (1, 2)
    \item $(\alpha \to (((\alpha \to \beta) \to \beta) \to (\neg\beta \to
    (\neg(\alpha \to \beta))))) \to ((\alpha \to ((\alpha \to \beta) \to
    \beta)) \to (\alpha \to (\neg\beta \to (\neg(\alpha \to \beta)))))$.
    \hfill (A2)
    \item $(\alpha \to ((\alpha \to \beta) \to \beta)) \to (\alpha \to
    (\neg\beta \to (\neg(\alpha \to \beta))))$. \hfill (3, 4)
    \item $\alpha \to ((\alpha \to \beta) \to \beta)$. \hfill
    (\Cref{thm:modus-ponens})
    \item $\alpha \to (\neg\beta \to \neg(\alpha \to \beta))$. \hfill (5, 6)
  \end{enumerate}
  Thus, we can conclude that $\vdash \alpha \to (\neg\beta \to \neg(\alpha \to
  \beta))$.
\end{proof}

\begin{theorem}[Deduction Theorem]
  \label{thm:deduction}
  Let $\Gamma$ be a set of formulas and let $\alpha$ and $\beta$ be formulas.
  If $\Gamma \cup \{\alpha\} \vdash \beta$, then
  $\Gamma \vdash \alpha \to \beta$.
\end{theorem}
\begin{proof}
  If $\beta \in \Lambda \cup \Gamma$, then we have
  $\Gamma \vdash \alpha \to \beta_k$ since
  $\vdash \beta_k \to (\alpha \to \beta_k)$.
  Furthermore, if $\beta = \alpha$, then we also have
  $\Gamma \vdash \alpha \to \beta$ since $\vdash \beta \to \beta$ by
  \Cref{thm:identity}.
  Thus, one only needs to consider the case that
  $\beta \notin \Lambda \cup \Gamma \cup \{\alpha\}$.

  Suppose that $(\beta_1, \beta_2, \dots, \beta_n)$ is a proof of $\beta$ from
  $\Gamma \cup \{\alpha\}$.
  For $1 \leq k \leq n$, we prove that $\Gamma \vdash \alpha \to \beta_k$ by
  induction on $k$.
  The induction basis holds for $k = 1$ since
  $\beta_1 \in \Lambda \cup \Gamma \cup \{\alpha\}$.
  For the induction step, let $k \geq 2$ and assume that
  $\Gamma \vdash \alpha \to \beta_\ell$ for $1 \leq \ell < k$.
  We have proved for the case that
  $\beta \in \Lambda \cup \Gamma \cup \{\alpha\}$, and thus we assume without
  loss of generality that there exist $1 \leq i < k$ and $1 \leq j < k$
  such that $\beta_j = \beta_i \to \beta_k$.
  Note that $\Gamma \vdash \alpha \to \beta_i$ and
  $\Gamma \vdash \alpha \to (\beta_i \to \beta_k)$
  hold by induction hypothesis.
  Therefore, since
  \begin{equation*}
    \vdash (\alpha \to (\beta_i \to \beta_k)) \to
    ((\alpha \to \beta_i) \to (\alpha \to \beta_k)),
  \end{equation*}
  we can conclude that $\Gamma \vdash \alpha \to \beta_k$,
  which completes the proof.
\end{proof}

\section{Soundness and Completeness}
\begin{theorem}
  Let $\alpha$ be a formula which consists of only the propositional variables
  $p_1, \dots, p_k$ and let $\tau$ be a truth assignment.
  Let $p_1^*, \dots, p_k^*$ be formulas such that for each
  $i \in \{1, \dots, k\}$,
  \begin{equation*}
    p_i^* =
    \begin{cases}
      p_i, & \text{if $\tau(p_i) = 1$} \\
      \neg p_i, & \text{if $\tau(p_i) = 0$}.
    \end{cases}
  \end{equation*}
  Furthermore, let $\alpha^*$ be the formula defined by
  \begin{equation*}
    \alpha^* =
    \begin{cases}
      \alpha, & \text{if $\tau(\alpha) = 1$} \\
      \neg \alpha, & \text{if $\tau(\alpha) = 0$}.
    \end{cases}
  \end{equation*}
  Then we have
  \begin{equation*}
    \{p_1^*, \dots, p_k^*\} \vdash \alpha^*.
  \end{equation*}
\end{theorem}
\begin{proof}
  The proof is by induction on the complexity of $\alpha$.
  It is straightforward that the theorem holds when $\alpha = p_i$ for some
  $i \in \{1, \dots, k\}$.

  Now suppose that $\{p_1^*, \dots, p_k^*\} \vdash \alpha^*$, and we prove
  that
  \begin{equation*}
    \{p_1^*, \dots, p_k^*\} \vdash \beta^*
  \end{equation*}
  with $\beta = \neg\alpha$.
  If $\tau(\alpha) = 0$, then $\tau(\beta) = 1$, and we have
  $\alpha^* = \neg\alpha = \beta^*$.
  Thus, $\{p_1^*, \dots, p_k^*\} \vdash \beta^*$.
  If $\tau(\alpha) = 1$, then $\tau(\beta) = 0$, and we have
  $\alpha^* = \alpha$ and $\beta^* = \neg\neg\alpha$.
  Since
  \begin{equation*}
    \{p_1^*, \dots, p_k^*\} \vdash \alpha
    \quad \text{and} \quad
    \vdash \alpha \to \neg\neg\alpha,
  \end{equation*}
  we have $\{p_1^*, \dots, p_k^*\} \vdash \beta^*$.

  Now suppose that $\{p_1^*, \dots, p_k^*\} \vdash \alpha^*$ and
  $\{p_1^*, \dots, p_k^*\} \vdash \beta^*$, and we prove that
  \begin{equation*}
    \{p_1^*, \dots, p_k^*\} \vdash \gamma^*
  \end{equation*}
  with $\gamma = \alpha \to \beta$.
  If $\tau(\alpha) = 0$, then $\tau(\gamma) = 1$, and we have
  $\alpha^* = \neg\alpha$ and $\gamma^* = \alpha \to \beta$.
  Since $\{p_1^*, \dots, p_k^*\} \vdash \neg\alpha$
  \begin{equation*}
    \{p_1^*, \dots, p_k^*\} \vdash \neg\alpha
    \quad \text{and} \quad
    \vdash \neg\alpha \to (\alpha \to \beta)
  \end{equation*}
  we have $\{p_1^*, \dots, p_k^*\} \vdash \gamma^*$.
  If $\tau(\beta) = 1$, then $\tau(\gamma) = 1$, and we have
  $\beta^* = \beta$ and $\gamma^* = \alpha \to \beta$.
  Since
  \begin{equation*}
    \{p_1^*, \dots, p_k^*\} \vdash \beta
    \quad \text{and} \quad
    \vdash \beta \to (\alpha \to \beta)
  \end{equation*}
  we have $\{p_1^*, \dots, p_k^*\} \vdash \gamma^*$.
  If $\tau(\alpha) = 1$ and $\tau(\beta) = 0$, then
  $\tau(\gamma) = 0$, and we have $\alpha^* = \alpha$, 
  $\beta^* = \neg\beta$ and $\gamma^* = \neg(\alpha \to \beta)$.
  Since
  \begin{equation*}
    \{p_1^*, \dots, p_k^*\} \vdash \alpha,
    \quad
    \{p_1^*, \dots, p_k^*\} \vdash \neg\beta,
    \quad \text{and} \quad
    \vdash \alpha \to (\neg\beta \to \neg(\alpha \to \beta)),
  \end{equation*}
  we have $\{p_1^*, \dots, p_k^*\} \vdash \gamma^*$, completing the proof.
\end{proof}